# baseURI: https://linked.data.gov.au/def/fsdf/common
# imports: http://purl.org/dc/terms/
# imports: http://www.w3.org/2004/02/skos/core

@prefix common: <https://linked.data.gov.au/def/fsdf/common/> .
@prefix dcterms: <http://purl.org/dc/terms/> .
@prefix owl: <http://www.w3.org/2002/07/owl#> .
@prefix rdf: <http://www.w3.org/1999/02/22-rdf-syntax-ns#> .
@prefix rdfs: <http://www.w3.org/2000/01/rdf-schema#> .
@prefix skos: <http://www.w3.org/2004/02/skos/core#> .
@prefix xsd: <http://www.w3.org/2001/XMLSchema#> .

<https://linked.data.gov.au/def/fsdf/common>
  a owl:Ontology ;
  a skos:ConceptScheme ;
  dcterms:created "2020-10-28"^^xsd:date ;
  dcterms:creator <https://orcid.org/0000-0002-3884-3420> ;
  dcterms:title "FSDF Common Codes"@en ;
  rdfs:comment "Common codelists used across multiple FSDF datasets"@en ;
  owl:imports dcterms: ;
  owl:imports <http://www.w3.org/2004/02/skos/core> ;
  skos:hasTopConcept common:abandoned ;
  skos:hasTopConcept common:below-ground ;
  skos:hasTopConcept common:decommissioned ;
  skos:hasTopConcept common:disused ;
  skos:hasTopConcept common:elevated ;
  skos:hasTopConcept common:non-operational ;
  skos:hasTopConcept common:on-ground ;
  skos:hasTopConcept common:operational ;
  skos:hasTopConcept common:other ;
  skos:hasTopConcept common:proposed ;
  skos:hasTopConcept common:under-construction ;
  skos:hasTopConcept common:unknown ;
  skos:prefLabel "FSDF Common Codes"@en ;
.
common:abandoned
  a skos:Concept ;
  skos:definition "Not in operation due to it being non-functional and operation is not scheduled to be restored"@en ;
  skos:prefLabel "Abandoned"@en ;
  skos:topConceptOf <https://linked.data.gov.au/def/fsdf/common> ;
.
common:below-ground
  a skos:Concept ;
  skos:definition "The entire feature is completely buried below the ground (terrain) surface."@en ;
  skos:prefLabel "Below ground"@en ;
  skos:topConceptOf <https://linked.data.gov.au/def/fsdf/common> ;
.
common:decommissioned
  a skos:Concept ;
  skos:definition "The infrastructure has been removed form service and has been or will be dismantled"@en ;
  skos:prefLabel "Decommissioned"@en ;
  skos:topConceptOf <https://linked.data.gov.au/def/fsdf/common> ;
.
common:disused
  a skos:Concept ;
  skos:definition "Temporarily not in operation due to it being non-functional and operation is scheduled to be restored"@en ;
  skos:prefLabel "Disused"@en ;
  skos:topConceptOf <https://linked.data.gov.au/def/fsdf/common> ;
.
common:elevated
  a skos:Concept ;
  skos:definition "Located above the ground (terrain) or the surface of the waterbody."@en ;
  skos:prefLabel "Elevated"@en ;
  skos:topConceptOf <https://linked.data.gov.au/def/fsdf/common> ;
.
common:non-operational
  a skos:Concept ;
  skos:definition "The feature is not currently operating"@en ;
  skos:prefLabel "Non-Operational"@en ;
  skos:topConceptOf <https://linked.data.gov.au/def/fsdf/common> ;
.
common:on-ground
  a skos:Concept ;
  skos:definition "Located on the ground (terrain) or the surface of the waterbody."@en ;
  skos:prefLabel "On ground"@en ;
  skos:topConceptOf <https://linked.data.gov.au/def/fsdf/common> ;
.
common:operational
  a skos:Concept ;
  skos:definition "Fully capable of operation"@en ;
  skos:prefLabel "Operational"@en ;
  skos:topConceptOf <https://linked.data.gov.au/def/fsdf/common> ;
.
common:operational-status
  a skos:Collection ;
  skos:member common:abandoned ;
  skos:member common:decommissioned ;
  skos:member common:disused ;
  skos:member common:non-operational ;
  skos:member common:operational ;
  skos:member common:other ;
  skos:member common:proposed ;
  skos:member common:under-construction ;
  skos:member common:unknown ;
  skos:prefLabel "Operational status"@en ;
.
common:other
  a skos:Concept ;
  skos:definition "The attribute value is known, but is not currently a valid member of the attribute range"@en ;
  skos:prefLabel "Other"@en ;
  skos:topConceptOf <https://linked.data.gov.au/def/fsdf/common> ;
.
common:proposed
  a skos:Concept ;
  skos:definition "Proposed infrastructure"@en ;
  skos:prefLabel "Proposed"@en ;
  skos:topConceptOf <https://linked.data.gov.au/def/fsdf/common> ;
.
common:relationship-to-ground
  a skos:Collection ;
  skos:member common:below-ground ;
  skos:member common:elevated ;
  skos:member common:on-ground ;
  skos:prefLabel "Relationship to ground"@en ;
.
common:under-construction
  a skos:Concept ;
  skos:definition "The feature is currently being built"@en ;
  skos:prefLabel "Under Construction"@en ;
  skos:topConceptOf <https://linked.data.gov.au/def/fsdf/common> ;
.
common:unknown
  a skos:Concept ;
  skos:definition "There is no information specified regarding the attribute value"@en ;
  skos:prefLabel "Unknown"@en ;
  skos:topConceptOf <https://linked.data.gov.au/def/fsdf/common> ;
.
